Rename Inst{_, _} to Instantaneous.{_, _}

src/ReactorModel/Determinism/Trivial.lean
@@ -14,52 +14,60 @@ section
 
 variable {s₁ : State} (triv : s₁.Trivial)
 
+namespace Instantaneous
+
+theorem Step.not_Trivial (e : s₁ ⇓ᵢ s₂) : ¬s₁.Trivial := by
+  by_contra ht
+  simp [State.Trivial, Partial.empty_iff] at ht
+  cases (Partial.mem_iff.mp e.allows_rcn.mem).choose_spec ▸ ht e.rcn  
+
+theorem Execution.trivial_eq : (s₁ ⇓ᵢ* s₂) → s₁ = s₂
+  | refl      => rfl
+  | trans e _ => absurd triv e.not_Trivial 
+
+theorem ClosedExecution.preserves_Trivial {e : s₁ ⇓| s₂} : s₂.Trivial := by
+  simp [State.Trivial, ←Equivalent.obj?_rcn_eq e.equiv, triv]
+
+theorem ClosedExecution.trivial_eq (e : s₁ ⇓| s₂) : s₁ = s₂ :=
+  e.exec.trivial_eq triv
+
+end Instantaneous
+
 theorem State.Advance.preserves_Trivial : (Advance s₁ s₂) → s₂.Trivial
   | mk .. => triv
 
 theorem AdvanceTag.preserves_Trivial (a : s₁ ⇓- s₂) : s₂.Trivial :=
   a.advance.preserves_Trivial triv
 
-theorem ClosedExecution.preserves_Trivial {e : s₁ ⇓| s₂} : s₂.Trivial := by
-  simp [State.Trivial, ←Equivalent.obj?_rcn_eq e.equiv, triv]
-
 theorem Step.preserves_Trivial : (s₁ ⇓ s₂) → s₂.Trivial
   | close e   => e.preserves_Trivial triv
   | advance a => a.preserves_Trivial triv
 
-theorem InstStep.not_Trivial (e : s₁ ⇓ᵢ s₂) : ¬s₁.Trivial := by
-  by_contra ht
-  simp [State.Trivial, Partial.empty_iff] at ht
-  cases (Partial.mem_iff.mp e.allows_rcn.mem).choose_spec ▸ ht e.rcn  
-
-theorem InstExecution.trivial_eq : (s₁ ⇓ᵢ* s₂) → s₁ = s₂
-  | refl      => rfl
-  | trans e _ => absurd triv e.not_Trivial 
-
-theorem ClosedExecution.trivial_eq (e : s₁ ⇓| s₂) : s₁ = s₂ :=
-  e.exec.trivial_eq triv
-
 end
 
-inductive AdvanceTag.RTC : State → State → Type
+namespace AdvanceTag 
+
+inductive RTC : State → State → Type
   | refl : RTC s s
   | trans : (s₁ ⇓- s₂) → (RTC s₂ s₃) → RTC s₁ s₃   
+
+theorem RTC.tag_le : (AdvanceTag.RTC s₁ s₂) → s₁.tag ≤ s₂.tag
+  | refl       => le_refl _
+  | trans a a' => le_trans (le_of_lt a.tag_lt) a'.tag_le
+
+theorem RTC.deterministic (ht : s₁.tag = s₂.tag) : 
+  (AdvanceTag.RTC s s₁) → (AdvanceTag.RTC s s₂) → s₁ = s₂
+  | refl,         refl         => rfl
+  | refl,         trans a a'   => absurd ht      (ne_of_lt $ lt_of_lt_of_le a.tag_lt a'.tag_le)
+  | trans a a',   refl         => absurd ht.symm (ne_of_lt $ lt_of_lt_of_le a.tag_lt a'.tag_le)
+  | trans a₁ a₁', trans a₂ a₂' => a₁'.deterministic ht (a₂.determinisic a₁ ▸ a₂')
+
+end AdvanceTag
 
 def to_AdvanceTagRTC (triv : s₁.Trivial) : (s₁ ⇓* s₂) → AdvanceTag.RTC s₁ s₂
   | refl                 => .refl
   | step (.advance a) e' => .trans a (e'.to_AdvanceTagRTC $ a.preserves_Trivial triv)
   | step (.close e) e'   => e.trivial_eq triv ▸ (e'.to_AdvanceTagRTC $ e.preserves_Trivial triv)
-
-theorem AdvanceTag.RTC.tag_le : (AdvanceTag.RTC s₁ s₂) → s₁.tag ≤ s₂.tag
-  | refl       => le_refl _
-  | trans a a' => le_trans (le_of_lt a.tag_lt) a'.tag_le
-
-theorem AdvanceTag.RTC.deterministic (ht : s₁.tag = s₂.tag) : 
-    (AdvanceTag.RTC s s₁) → (AdvanceTag.RTC s s₂) →  s₁ = s₂
-  | refl,         refl         => rfl
-  | refl,         trans a a'   => absurd ht      (ne_of_lt $ lt_of_lt_of_le a.tag_lt a'.tag_le)
-  | trans a a',   refl         => absurd ht.symm (ne_of_lt $ lt_of_lt_of_le a.tag_lt a'.tag_le)
-  | trans a₁ a₁', trans a₂ a₂' => a₁'.deterministic ht (a₂.determinisic a₁ ▸ a₂')
 
 theorem trivial_deterministic 
     (triv : ¬s.Nontrivial) (e₁ : s ⇓* s₁) (e₂ : s ⇓* s₂) (ht : s₁.tag = s₂.tag) : s₁ = s₂ :=
