src/ReactorModel/Execution/Trace.lean
@@ -3,71 +3,75 @@ import ReactorModel.Execution.State
 open Classical
 
 namespace Execution
+namespace Instantaneous
+namespace Step
 
-inductive InstStep.Skip : State → State → Type  
+inductive Skip : State → State → Type  
   | mk : (s.Allows rcn) → (¬s.Triggers rcn) → Skip s (s.record rcn)
 
-notation s₁:max " ⇓ₛ " s₂:max => InstStep.Skip s₁ s₂
+notation s₁:max " ⇓ₛ " s₂:max => Skip s₁ s₂
 
-def InstStep.Skip.rcn : (s₁ ⇓ₛ s₂) → ID
+def Skip.rcn : (s₁ ⇓ₛ s₂) → ID
   | mk (rcn := rcn) .. => rcn
 
-def InstStep.Skip.allows_rcn : (e : s₁ ⇓ₛ s₂) → s₁.Allows e.rcn
+def Skip.allows_rcn : (e : s₁ ⇓ₛ s₂) → s₁.Allows e.rcn
   | mk h .. => h
 
-def InstStep.Skip.not_triggers : (e : s₁ ⇓ₛ s₂) → ¬s₁.Triggers e.rcn
+def Skip.not_triggers : (e : s₁ ⇓ₛ s₂) → ¬s₁.Triggers e.rcn
   | mk _ h => h
 
-inductive InstStep.Exec : State → State → Type  
+inductive Exec : State → State → Type  
   | mk : (s.Allows rcn) → (s.Triggers rcn) → Exec s (s.exec rcn |>.record rcn)
 
-notation s₁:max " ⇓ₑ " s₂:max => InstStep.Exec s₁ s₂
+notation s₁:max " ⇓ₑ " s₂:max => Exec s₁ s₂
 
-def InstStep.Exec.rcn : (s₁ ⇓ₑ s₂) → ID
+def Exec.rcn : (s₁ ⇓ₑ s₂) → ID
   | mk (rcn := rcn) .. => rcn
 
-def InstStep.Exec.allows_rcn : (e : s₁ ⇓ₑ s₂) → s₁.Allows e.rcn
+def Exec.allows_rcn : (e : s₁ ⇓ₑ s₂) → s₁.Allows e.rcn
   | mk h .. => h
 
-inductive InstStep (s₁ s₂ : State)
-  | skip (e : InstStep.Skip s₁ s₂)
-  | exec (e : InstStep.Exec s₁ s₂)
+inductive _root_.Execution.Instantaneous.Step (s₁ s₂ : State)
+  | skip (e : Skip s₁ s₂)
+  | exec (e : Exec s₁ s₂)
 
-notation s₁:max " ⇓ᵢ " s₂:max => InstStep s₁ s₂
+notation s₁:max " ⇓ᵢ " s₂:max => Step s₁ s₂
 
-def InstStep.rcn : (s₁ ⇓ᵢ s₂) → ID
+def rcn : (s₁ ⇓ᵢ s₂) → ID
   | skip e | exec e => e.rcn
 
-def InstStep.allows_rcn : (e : s₁ ⇓ᵢ s₂) → s₁.Allows e.rcn
+def allows_rcn : (e : s₁ ⇓ᵢ s₂) → s₁.Allows e.rcn
   | skip e | exec e => e.allows_rcn
+
+end Step
 
 -- TODO?: Once all else is settled, return this to being only transitive but not reflexive.
 --        Then you can remove the `fresh` condiction on `ClosedExecution`.
-inductive InstExecution : State → State → Type
-  | refl : InstExecution s s
-  | trans : (s₁ ⇓ᵢ s₂) → (InstExecution s₂ s₃) → InstExecution s₁ s₃
+inductive Execution : State → State → Type
+  | refl : Execution s s
+  | trans : (s₁ ⇓ᵢ s₂) → (Execution s₂ s₃) → Execution s₁ s₃
 
-notation s₁:max " ⇓ᵢ* " s₂:max => InstExecution s₁ s₂
+notation s₁:max " ⇓ᵢ* " s₂:max => Execution s₁ s₂
 
-def InstExecution.rcns : (s₁ ⇓ᵢ* s₂) → List ID
+def Execution.rcns : (s₁ ⇓ᵢ* s₂) → List ID
   | refl => []
   | trans hd tl => hd.rcn :: tl.rcns
-
-open State (Closed)
 
 structure ClosedExecution (s₁ s₂ : State) where  
   exec   : s₁ ⇓ᵢ* s₂
   fresh  : s₁.progress = ∅ 
-  closed : Closed s₂
+  closed : s₂.Closed
   
 notation s₁:max " ⇓| " s₂:max => ClosedExecution s₁ s₂
 
 abbrev ClosedExecution.rcns (e : s₁ ⇓| s₂) : List ID :=
   e.exec.rcns
 
+end Instantaneous
+
 -- Note: We don't clear the ports here.
 structure AdvanceTag (s₁ s₂ : State) where
-  closed : Closed s₁ 
+  closed : s₁.Closed 
   advance : s₁.Advance s₂
 
 notation s₁:max " ⇓- " s₂:max => AdvanceTag s₁ s₂
